Generated wp works partially. Experimentally using is in tool.

src/main/isabelle/Cert_Codegen.thy
@@ -2,6 +2,10 @@ theory Cert_Codegen
   imports Main ML_Term_Antiquot
 begin
 
+definition "list_last list xs x = (xs@[x] = list)"
+lemma list_lastI: "(xs@[x] == list) \<Longrightarrow> list_last list xs x"
+  unfolding list_last_def by simp
+
 definition "assert_equals a b = (a=b)"
 lemma assert_equals_refl: "assert_equals a a" unfolding assert_equals_def by simp
 definition [simp]: "assert_string_neq (a::string) b = (a \<noteq> b)"
@@ -14,12 +18,15 @@ lemma constant_function_absI: "constant_function (%z::'a. y) y"
 ML_file "cert_codegen.ML"
 
 setup \<open>
-  Cert_Codegen.add_specs [
-    Cert_Codegen.constant_function_spec,
-    Cert_Codegen.assert_equals_func_spec,
-    Cert_Codegen.string_concat_func_spec,
-    Cert_Codegen.assert_string_neq_func_spec,
-    Cert_Codegen.NO_MATCH_func_spec]
+let open Cert_Codegen in
+  add_specs [
+    list_last_spec,
+    constant_function_spec,
+    assert_equals_func_spec,
+    string_concat_func_spec,
+    assert_string_neq_func_spec,
+    NO_MATCH_func_spec]
+end
 \<close>
 
 end
